instantiated all modules

Structures/BlockedAMQ/BlockedAMQ.v
@@ -24,6 +24,17 @@ From ProbHash.Computation
 From ProbHash.Core
      Require Import Hash HashVec FixedList FixedMap.
 
+From ProbHash.BloomFilter
+     Require Import BloomFilter_Definitions.
+
+From ProbHash.CountingBloomFilter
+     Require Import CountingBloomFilter_Definitions.
+
+From ProbHash.QuotientFilter
+     Require Import QuotientFilter_Definitions.
+
+
+
 Lemma index_enum_simpl y: ((index_enum y)) = (index_enum [finType of y]).
 Proof.
     by rewrite /index_enum //= /[finType of _] //=; case: y => //=.
@@ -70,9 +81,9 @@ Module Type AMQHASH.
 
 
       Axiom AMQHash_hashstate_available_capacityW: forall n m, m <= n ->
-          AMQHash_hashstate_valid hashstate ->
-          AMQHash_hashstate_available_capacity hashstate n ->
-          AMQHash_hashstate_available_capacity hashstate m.
+                                                               AMQHash_hashstate_valid hashstate ->
+                                                               AMQHash_hashstate_available_capacity hashstate n ->
+                                                               AMQHash_hashstate_available_capacity hashstate m.
 
       Axiom AMQHash_hashstate_available_capacity_decr: forall l key value,
           AMQHash_hashstate_valid hashstate ->
@@ -89,7 +100,7 @@ Module Type AMQHASH.
       Axiom  AMQHash_hashstate_add_contains_base: forall (key: AMQHashKey) (value: AMQHashValue p),
           AMQHash_hashstate_valid hashstate ->
           AMQHash_hashstate_available_capacity hashstate 1 ->
-        AMQHash_hashstate_contains (AMQHash_hashstate_put  hashstate key value) key value.
+          AMQHash_hashstate_contains (AMQHash_hashstate_put  hashstate key value) key value.
 
       Axiom AMQHash_hashstate_add_valid_preserve: forall (key: AMQHashKey) (value: AMQHashValue p), 
           AMQHash_hashstate_valid hashstate ->
@@ -106,17 +117,17 @@ Module Type AMQHASH.
 
     
     Axiom  AMQHash_hash_unseen_insert_eqE: forall (hashstate hashstate': AMQHash p) (key: AMQHashKey) (value: AMQHashValue p),
-          AMQHash_hashstate_unseen hashstate key -> hashstate' = AMQHash_hashstate_put hashstate key value ->
-          d[ AMQHash_hash hashstate key ] (hashstate', value) = AMQHash_probability p.
+        AMQHash_hashstate_unseen hashstate key -> hashstate' = AMQHash_hashstate_put hashstate key value ->
+        d[ AMQHash_hash hashstate key ] (hashstate', value) = AMQHash_probability p.
 
     Axiom  AMQHash_hash_unseen_insert_neqE: forall (hashstate hashstate': AMQHash p) (key: AMQHashKey) (value: AMQHashValue p),
-          AMQHash_hashstate_unseen hashstate key -> hashstate' != AMQHash_hashstate_put hashstate key value ->
-          d[ AMQHash_hash hashstate key ] (hashstate', value) = 0.
+        AMQHash_hashstate_unseen hashstate key -> hashstate' != AMQHash_hashstate_put hashstate key value ->
+        d[ AMQHash_hash hashstate key ] (hashstate', value) = 0.
 
     Axiom AMQHash_hash_seen_insertE: forall (hashstate hashstate': AMQHash p) (key: AMQHashKey) (value value': AMQHashValue p),
         AMQHash_hashstate_contains hashstate key value ->
         d[ AMQHash_hash hashstate key ] (hashstate', value') = ((hashstate' == hashstate) && (value' == value)).
-        
+    
   End AMQHash.    
 End AMQHASH.
 
@@ -127,11 +138,11 @@ Module AMQHashProperties (AMQHash: AMQHASH).
     Variable p: AMQHashParams. 
     
     Lemma AMQHash_hash_unseen_simplE (hashstate: AMQHash p) key value f :
-        AMQHash_hashstate_unseen hashstate key ->
-        (\sum_(hashstate' in [finType of AMQHash p])
-         (d[ AMQHash_hash hashstate key ] (hashstate', value) *R* (f hashstate'))) =
-        ((AMQHash_probability p) *R*
-         (f (AMQHash_hashstate_put hashstate key value))).
+      AMQHash_hashstate_unseen hashstate key ->
+      (\sum_(hashstate' in [finType of AMQHash p])
+        (d[ AMQHash_hash hashstate key ] (hashstate', value) *R* (f hashstate'))) =
+      ((AMQHash_probability p) *R*
+       (f (AMQHash_hashstate_put hashstate key value))).
     Proof.
       move=> Hall.
       rewrite (bigID (fun hashstate' => hashstate' == (AMQHash_hashstate_put hashstate key value))) //=.
@@ -158,11 +169,9 @@ Module Type AMQ (AMQHash: AMQHASH).
     Variable p: AMQStateParams.
     Variable h: AMQHash.AMQHashParams.
 
-    Parameter AMQ_hash_vec_size: AMQStateParams -> nat.
-    
     Parameter AMQ_add_internal: AMQState p -> AMQHash.AMQHashValue h -> AMQState p.
     Parameter AMQ_query_internal: AMQState p -> AMQHash.AMQHashValue h -> bool.
-    Parameter AMQ_available_capacity: AMQState p -> nat -> bool.
+    Parameter AMQ_available_capacity: AMQHash.AMQHashParams -> AMQState p -> nat -> bool.
     Parameter AMQ_valid: AMQState p -> bool.
 
     Axiom AMQ_new: AMQState p.
@@ -173,29 +182,29 @@ Module Type AMQ (AMQHash: AMQHASH).
       Variable amq: AMQState p.
 
       Axiom AMQ_available_capacityW: forall  n m,
-          AMQ_valid amq -> m <= n -> AMQ_available_capacity amq n -> AMQ_available_capacity amq m.
+          AMQ_valid amq -> m <= n -> AMQ_available_capacity h amq n -> AMQ_available_capacity h amq m.
 
-    Axiom AMQ_add_query_base: forall (amq: AMQState p) inds,
-        AMQ_valid amq -> AMQ_available_capacity amq 1 ->
-        AMQ_query_internal (AMQ_add_internal amq inds) inds.
+      Axiom AMQ_add_query_base: forall (amq: AMQState p) inds,
+          AMQ_valid amq -> AMQ_available_capacity h amq 1 ->
+          AMQ_query_internal (AMQ_add_internal amq inds) inds.
 
-    Axiom AMQ_add_valid_preserve: forall (amq: AMQState p) inds,
-        AMQ_valid amq -> AMQ_available_capacity amq 1 ->
-        AMQ_valid (AMQ_add_internal amq inds).
+      Axiom AMQ_add_valid_preserve: forall (amq: AMQState p) inds,
+          AMQ_valid amq -> AMQ_available_capacity h amq 1 ->
+          AMQ_valid (AMQ_add_internal amq inds).
 
-    Axiom AMQ_add_query_preserve: forall (amq: AMQState p) inds inds',
-        AMQ_valid amq -> AMQ_available_capacity amq 1 -> AMQ_query_internal amq inds ->
-        AMQ_query_internal (AMQ_add_internal amq inds') inds.
+      Axiom AMQ_add_query_preserve: forall (amq: AMQState p) inds inds',
+          AMQ_valid amq -> AMQ_available_capacity h amq 1 -> AMQ_query_internal amq inds ->
+          AMQ_query_internal (AMQ_add_internal amq inds') inds.
 
-    Axiom AMQ_add_capacity_decr: forall (amq: AMQState p) inds l,
-        AMQ_valid amq -> AMQ_available_capacity amq l.+1 ->
-        AMQ_available_capacity (AMQ_add_internal amq inds) l.
-    
-    Axiom AMQ_query_valid_preserve: forall (amq: AMQState p) inds,
-        AMQ_valid amq -> AMQ_valid (AMQ_add_internal amq inds).
+      Axiom AMQ_add_capacity_decr: forall (amq: AMQState p) inds l,
+          AMQ_valid amq -> AMQ_available_capacity h amq l.+1 ->
+          AMQ_available_capacity h (AMQ_add_internal amq inds) l.
+      
+      Axiom AMQ_query_valid_preserve: forall (amq: AMQState p) inds,
+          AMQ_valid amq -> AMQ_valid (AMQ_add_internal amq inds).
 
-    Axiom AMQ_query_capacity_preserve: forall (amq: AMQState p) inds l,
-        AMQ_valid amq -> AMQ_available_capacity amq l.+1 -> AMQ_available_capacity (AMQ_add_internal amq inds) l.
+      Axiom AMQ_query_capacity_preserve: forall (amq: AMQState p) inds l,
+          AMQ_valid amq -> AMQ_available_capacity h amq l.+1 -> AMQ_available_capacity h (AMQ_add_internal amq inds) l.
 
     End DeterministicProperties.
   End AMQ.
@@ -217,24 +226,24 @@ Module AMQOperations (AmqHash: AMQHASH) (Amq: AMQ AmqHash) .
     Definition AMQ_add (amq: AMQState s)   (hashes: AMQHash h) (value: AMQHashKey) :
       Comp [finType of (AMQHash h) * AMQState s] :=
       hash_res <-$ (AMQHash_hash  hashes value);
-      let (new_hashes, hash_vec) := hash_res in
-      let new_amq := AMQ_add_internal amq hash_vec in
-      ret (new_hashes, new_amq).
+        let (new_hashes, hash_vec) := hash_res in
+        let new_amq := AMQ_add_internal amq hash_vec in
+        ret (new_hashes, new_amq).
 
     Definition AMQ_query (amq: AMQState s)   (hashes: AMQHash h) (value: AMQHashKey) :
       Comp [finType of (AMQHash h) * bool] :=
       hash_res <-$ (AMQHash_hash  hashes value);
-      let (new_hashes, hash_vec) := hash_res in
-      let new_amq := AMQ_query_internal amq hash_vec in
-      ret (new_hashes, new_amq).
+        let (new_hashes, hash_vec) := hash_res in
+        let new_amq := AMQ_query_internal amq hash_vec in
+        ret (new_hashes, new_amq).
     
 
     Definition AMQ_add_multiple  hsh_0 bf_0 values :=
-    @foldr _ (Comp [finType of AMQHash h * AMQState s])
-           (fun val hsh_bf =>
-              res_1 <-$ hsh_bf;
-                let (hsh, bf) := res_1 in
-                AMQ_add bf hsh val) (ret (hsh_0, bf_0)) values.
+      @foldr _ (Comp [finType of AMQHash h * AMQState s])
+             (fun val hsh_bf =>
+                res_1 <-$ hsh_bf;
+                  let (hsh, bf) := res_1 in
+                  AMQ_add bf hsh val) (ret (hsh_0, bf_0)) values.
   End Operations.
 
   Section Properties.
@@ -245,21 +254,21 @@ Module AMQOperations (AmqHash: AMQHASH) (Amq: AMQ AmqHash) .
     Variable amq: AMQState s.
 
     Lemma AMQ_add_multiple_properties_preserve  ( cbf': AMQState s)  values inds' l m:
-            length values == l -> AMQ_valid amq ->  AMQ_available_capacity amq (l + m) ->
-            (P[ AMQ_add_multiple hashes amq values === (inds', cbf')] != 0) ->
-            AMQ_valid cbf' && AMQ_available_capacity cbf' m.
-          Proof.
-            move=>/eqP <-; clear l.
-            elim: values m amq cbf' inds' => [| x xs Hxs] m cbf cbf' inds' Hvalid Havail //=; comp_normalize;
-            first by move=>/bool_neq0_true; rewrite xpair_eqE=>/andP[_ /eqP -> ]; apply/andP => //=.
-            exchange_big_outwards 2 => //=; comp_simplify_n 1; comp_possible_decompose.
-            move=> cbf'' inds'' Hind Haddm Hhash /bool_neq0_true/eqP ->.
-            move: Havail => //=; rewrite addSn -addnS => Havail.
-            move: (@Hxs m.+1 cbf inds'' cbf'' Hvalid Havail Haddm); clear Hxs Haddm => /andP [Hvalid' Hfree'].
-            apply/andP;split.
-            apply AMQ_add_valid_preserve => //=; apply AMQ_available_capacityW with (n:= m.+1) => //=.
-            apply AMQ_add_capacity_decr => //=.
-          Qed.
+      length values == l -> AMQ_valid amq ->  AMQ_available_capacity h amq (l + m) ->
+      (P[ AMQ_add_multiple hashes amq values === (inds', cbf')] != 0) ->
+      AMQ_valid cbf' && AMQ_available_capacity h cbf' m.
+    Proof.
+      move=>/eqP <-; clear l.
+      elim: values m amq cbf' inds' => [| x xs Hxs] m cbf cbf' inds' Hvalid Havail //=; comp_normalize;
+                                         first by move=>/bool_neq0_true; rewrite xpair_eqE=>/andP[_ /eqP -> ]; apply/andP => //=.
+      exchange_big_outwards 2 => //=; comp_simplify_n 1; comp_possible_decompose.
+      move=> cbf'' inds'' Hind Haddm Hhash /bool_neq0_true/eqP ->.
+      move: Havail => //=; rewrite addSn -addnS => Havail.
+      move: (@Hxs m.+1 cbf inds'' cbf'' Hvalid Havail Haddm); clear Hxs Haddm => /andP [Hvalid' Hfree'].
+      apply/andP;split.
+      apply AMQ_add_valid_preserve => //=; apply AMQ_available_capacityW with (n:= m.+1) => //=.
+      apply AMQ_add_capacity_decr => //=.
+    Qed.
 
   End Properties.
 
@@ -271,7 +280,7 @@ Module AMQOperations (AmqHash: AMQHASH) (Amq: AMQ AmqHash) .
     Variable amq: AMQState s.
 
     Lemma AMQ_add_multiple_query_preserve  ( amq': AMQState s)  values inds inds' l:
-      length values == l -> AMQ_valid amq ->  AMQ_available_capacity amq l -> AMQ_query_internal amq inds ->
+      length values == l -> AMQ_valid amq ->  AMQ_available_capacity h amq l -> AMQ_query_internal amq inds ->
       (P[ AMQ_add_multiple hashes amq values === (inds', amq')] != 0) ->
       @AMQ_query_internal _ h amq' inds.
     Proof.
@@ -284,7 +293,7 @@ Module AMQOperations (AmqHash: AMQHASH) (Amq: AMQ AmqHash) .
       move: (@AMQ_add_multiple_properties_preserve h s hashes cbf inds'' xs cbf'' (length xs) 1 (eq_refl (length xs)) Hvalid Havail Haddm) => /andP [Hvalid' Hcap'].
       apply AMQ_add_query_preserve => //=.
       eapply Hxs with (amq:= cbf) (inds':= cbf'') => //=.
-      by apply AMQ_available_capacityW with (n:= length xs + 1) => //=; last  rewrite addn1.
+        by apply AMQ_available_capacityW with (n:= length xs + 1) => //=; last  rewrite addn1.
     Qed.
     
   End Query.
@@ -318,15 +327,15 @@ Module AMQOperations (AmqHash: AMQHASH) (Amq: AMQ AmqHash) .
           first by move: Huns => //=/andP[ -> /andP [ _ ->]  ].
         move: (@Hxs y m.+1 cbf cbf'' hshs hsh'' Hvalid H1 H2 H3 Haddm) => /andP [/andP [Hcap' Huns'] Hvalid'].
         move: (@Hxs x m.+1 cbf cbf'' hshs hsh'' Hvalid H1' H2 H3' Haddm) => /andP [/andP [_ Hunsx'] _].
-      case Heq: (hshs' != AMQHash_hashstate_put hsh'' y y').
+        case Heq: (hshs' != AMQHash_hashstate_put hsh'' y y').
       - by move: (AMQHash_hash_unseen_insert_neqE Huns' Heq) Hhash => -> //= /eqP //=.
       - move/Bool.negb_false_iff: Heq => /eqP ->.
         apply /andP; split; first apply/andP; first split => //=.
-        by apply  AMQHash_hashstate_available_capacity_decr => //=.
-        apply AMQHash_hashstate_unseenE with (hashstate:=hsh'') (key' := y) (value':=y') => //=.
-        by move: Huni => //=/andP[]; rewrite in_cons Bool.negb_orb => /andP[].
-        apply AMQHash_hashstate_add_valid_preserve => //=.
-        apply AMQHash_hashstate_available_capacityW with (n:=m.+1) => //=.
+          by apply  AMQHash_hashstate_available_capacity_decr => //=.
+          apply AMQHash_hashstate_unseenE with (hashstate:=hsh'') (key' := y) (value':=y') => //=.
+            by move: Huni => //=/andP[]; rewrite in_cons Bool.negb_orb => /andP[].
+            apply AMQHash_hashstate_add_valid_preserve => //=.
+            apply AMQHash_hashstate_available_capacityW with (n:=m.+1) => //=.
     Qed.
   End HashProperties.
 
@@ -361,7 +370,7 @@ Module AMQOperations (AmqHash: AMQHASH) (Amq: AMQ AmqHash) .
         }
 
         have H3: (all (AMQHash_hashstate_unseen hshs) ys). {
-          by move: Huns => //= /andP[].
+            by move: Huns => //= /andP[].
         }
         move: Hhash (@Hxs x cbf cbf'' hshs hsh'' Hvalid H1' H2 H3 Hcont  Haddm).
         have Huniys: (uniq (y :: ys)); first by move: Huni => //=.
@@ -371,16 +380,16 @@ Module AMQOperations (AmqHash: AMQHASH) (Amq: AMQ AmqHash) .
         case Hneq: (hshs' != AMQHash_hashstate_put hsh'' y y').
         {
           - move: Huns => //=/andP[Hyun Huns].
-            by move: (AMQHash_hash_unseen_insert_neqE Hunsy  Hneq) -> => /eqP //=.
+              by move: (AMQHash_hash_unseen_insert_neqE Hunsy  Hneq) -> => /eqP //=.
         }
         {
           - move/Bool.negb_true_iff: Hneq; rewrite Bool.negb_involutive => /eqP -> Hn0 Hcontains.  
             apply AMQHash_hashstate_add_contains_preserve => //=.
-            by move: Huni => //= /andP []; rewrite in_cons Bool.negb_orb => /andP[].
+              by move: Huni => //= /andP []; rewrite in_cons Bool.negb_orb => /andP[].
         }        
     Qed.
 
-    End HashProperties.
+  End HashProperties.
 
   Section FalseNegatives.
     Variable h : AMQHashParams.
@@ -388,18 +397,18 @@ Module AMQOperations (AmqHash: AMQHASH) (Amq: AMQ AmqHash) .
 
     Theorem AMQ_no_false_negatives (hashes: AmqHash.AMQHash h)  (amq: AMQState s) l x xs:
       uniq (x :: xs) -> length xs == l ->
-      AMQ_valid amq -> AMQ_available_capacity amq l.+1 ->
+      AMQ_valid amq -> AMQ_available_capacity h amq l.+1 ->
 
       AmqHash.AMQHash_hashstate_valid hashes ->
       AmqHash.AMQHash_hashstate_available_capacity hashes l.+1 ->
 
       all (AmqHash.AMQHash_hashstate_unseen hashes) (x::xs) ->
       (d[ res1 <-$ AMQ_add amq hashes x;
-          let '(hsh1, amq1) := res1 in
-          res2 <-$ AMQ_add_multiple hsh1 amq1 xs;
-            let '(hsh2, amq2) := res2 in
-            res3 <-$ AMQ_query amq2 hsh2 x;
-              ret (snd res3) ] true) = (1 %R).
+            let '(hsh1, amq1) := res1 in
+            res2 <-$ AMQ_add_multiple hsh1 amq1 xs;
+              let '(hsh2, amq2) := res2 in
+              res3 <-$ AMQ_query amq2 hsh2 x;
+                ret (snd res3) ] true) = (1 %R).
     Proof.
       move=> Huniq Hlen Hamqvalid Hamqavail Hvalid Havail Hall.
       comp_normalize; comp_simplify_n 2.
@@ -411,23 +420,23 @@ Module AMQOperations (AmqHash: AMQHASH) (Amq: AMQ AmqHash) .
 
       under eq_bigr => hshs' _. {
         under eq_bigr => amq' _; first under eq_bigr => ind _; first under eq_bigr => hshs'' _;
-        first under eq_rsum_ne0  => ind' Hn0.
+                                                                                        first under eq_rsum_ne0  => ind' Hn0.
 
         have Hvalidamqin: (AMQ_valid (AMQ_add_internal amq ind)). {
           apply AMQ_add_valid_preserve=>//=.          
-          by apply AMQ_available_capacityW with (n:=l.+1)=>//=.
+            by apply AMQ_available_capacityW with (n:=l.+1)=>//=.
         }
         have Hvalidin: (AmqHash.AMQHash_hashstate_valid (AmqHash.AMQHash_hashstate_put hashes x ind)).
         {
           apply AmqHash.AMQHash_hashstate_add_valid_preserve => //=.
-          by apply AmqHash.AMQHash_hashstate_available_capacityW with (n:=l.+1)=>//=.
+            by apply AmqHash.AMQHash_hashstate_available_capacityW with (n:=l.+1)=>//=.
         }
-        have Havailamqin: (AMQ_available_capacity (AMQ_add_internal amq ind) l); first
+        have Havailamqin: (AMQ_available_capacity h (AMQ_add_internal amq ind) l); first
           by apply AMQ_add_capacity_decr => //=.
 
         have Hqueryamqin: (AMQ_query_internal (AMQ_add_internal amq ind) ind). {
           apply AMQ_add_query_base => //=.
-          by apply AMQ_available_capacityW with (n:=l.+1)=>//=.
+            by apply AMQ_available_capacityW with (n:=l.+1)=>//=.
         }
 
         have Hin: (AMQHash_hashstate_contains hshs' x ind). {
@@ -455,7 +464,7 @@ Module AMQOperations (AmqHash: AMQHASH) (Amq: AMQ AmqHash) .
         rewrite mulRA [_ *R* (_ && _)]mulRC -!mulRA.
 
         rewrite -RIneq.INR_IZR_INZ boolR_distr.
-        by over. by over. by over. by over. by over.
+          by over. by over. by over. by over. by over.
       }
       comp_normalize.
       under_all ltac:(rewrite mulRC -!mulRA ).
@@ -465,7 +474,7 @@ Module AMQOperations (AmqHash: AMQHASH) (Amq: AMQ AmqHash) .
         rewrite -(@rsum_pred_demote [finType of AmqHash.AMQHash h]) big_pred1_eq; over => //=.
         rewrite index_enum_simpl //=.
         rewrite -(@rsum_pred_demote [finType of AmqHash.AMQHashValue h]) big_pred1_eq.
-        by over. by over. by over.
+          by over. by over. by over.
       }
       under_all ltac:(rewrite mulRC [(_ %R) *R* _]mulRC -!mulRA).
       under eq_bigr => hshs' _. { 
@@ -477,14 +486,14 @@ Module AMQOperations (AmqHash: AMQHASH) (Amq: AMQ AmqHash) .
         have Hvalidin: (AmqHash.AMQHash_hashstate_valid (AmqHash.AMQHash_hashstate_put hashes x ind)).
         {
           apply AmqHash.AMQHash_hashstate_add_valid_preserve => //=.
-          by apply AmqHash.AMQHash_hashstate_available_capacityW with (n:=l.+1)=>//=.
+            by apply AmqHash.AMQHash_hashstate_available_capacityW with (n:=l.+1)=>//=.
         }
-        have Havailamqin: (AMQ_available_capacity (AMQ_add_internal amq ind) l); first
+        have Havailamqin: (AMQ_available_capacity h (AMQ_add_internal amq ind) l); first
           by apply AMQ_add_capacity_decr => //=.
 
         have Hqueryamqin: (AMQ_query_internal (AMQ_add_internal amq ind) ind). {
           apply AMQ_add_query_base => //=.
-         by apply AMQ_available_capacityW with (n:=l.+1)=>//=.
+            by apply AMQ_available_capacityW with (n:=l.+1)=>//=.
         }
 
         have Hqueryint: (AMQ_query_internal amq' ind). {
@@ -496,13 +505,13 @@ Module AMQOperations (AmqHash: AMQHASH) (Amq: AMQ AmqHash) .
                  (amq':=amq')
                  (inds':=hshs')
                  (l:=l)
-                 => //=.
+          => //=.
         }
         rewrite Hqueryint eq_refl //= mul1R.
 
-        by over.
-        by over.
-        by over.
+          by over.
+            by over.
+              by over.
       }
       move=>//=.
 
@@ -513,15 +522,15 @@ Module AMQOperations (AmqHash: AMQHASH) (Amq: AMQ AmqHash) .
       under eq_bigr => i Hi.
       rewrite -index_enum_simpl.
       suff ->:  \sum_(i0 in  AmqHash.AMQHash h)
-         \sum_(i1 in   AMQState s)
-            P[ AMQ_add_multiple
-                 (AmqHash.AMQHash_hashstate_put hashes x i)
-                 (AMQ_add_internal amq i) xs === 
-                 (i0, i1)] = 1;
+           \sum_(i1 in   AMQState s)
+           P[ AMQ_add_multiple
+                (AmqHash.AMQHash_hashstate_put hashes x i)
+                (AMQ_add_internal amq i) xs === 
+                (i0, i1)] = 1;
         last first; last rewrite mulR1; last by over.
-      by rewrite -rsum_split //=; apply FDist.f1.
-      move=> //=.
-      by rewrite AmqHash.AMQHash_hash_prob_valid.
+        by rewrite -rsum_split //=; apply FDist.f1.
+        move=> //=.
+          by rewrite AmqHash.AMQHash_hash_prob_valid.
     Qed.
   End FalseNegatives.
 
@@ -544,18 +553,18 @@ Module Type AMQProperties (AmqHash: AMQHASH) (AbstractAMQ: AMQ AmqHash) .
       forall (l:nat_eqType) (x:AMQHashKey) (xs: seq AMQHashKey),
         uniq (x :: xs) -> length xs == l ->
 
-        AMQ_valid amq -> AMQ_available_capacity amq l.+1 ->
+        AMQ_valid amq -> AMQ_available_capacity h amq l.+1 ->
 
         AMQHash_hashstate_valid hashes ->
         AMQHash_hashstate_available_capacity hashes l.+1 ->
 
         all (AMQHash_hashstate_unseen hashes) (x::xs) ->
         (d[ res1 <-$ AMQ_add amq hashes x;
-          let '(hsh1, amq1) := res1 in
-          res2 <-$ AMQ_add_multiple hsh1 amq1 xs;
-            let '(hsh2, amq2) := res2 in
-            res3 <-$ AMQ_query amq2 hsh2 x;
-              ret (snd res3) ] true) = (1 %R).
+              let '(hsh1, amq1) := res1 in
+              res2 <-$ AMQ_add_multiple hsh1 amq1 xs;
+                let '(hsh2, amq2) := res2 in
+                res3 <-$ AMQ_query amq2 hsh2 x;
+                  ret (snd res3) ] true) = (1 %R).
 
     Axiom AMQ_false_positives_rate: forall  l value (values: seq _),
         length values == l ->
@@ -564,7 +573,7 @@ Module Type AMQProperties (AmqHash: AMQHASH) (AbstractAMQ: AMQ AmqHash) .
         AMQHash_hashstate_available_capacity hashes (l.+1) ->
 
 
-        AMQ_available_capacity (AMQ_new s) l.+1 ->
+        AMQ_available_capacity h (AMQ_new s) l.+1 ->
         all (AMQHash_hashstate_unseen hashes) (value::values) ->
         uniq (value::values) ->
         d[ 
@@ -593,20 +602,20 @@ Module Type AMQMAP (AmqHash: AMQHASH) (A: AMQ AmqHash) (B: AMQ AmqHash).
     Variable h: AmqHash.AMQHashParams.
 
     Axiom AMQ_map_validE: forall (a: A.AMQState p), A.AMQ_valid a ->
-                                                        B.AMQ_valid (AMQ_state_map a).
-    Axiom AMQ_map_capacityE: forall (a: A.AMQState p) l, A.AMQ_available_capacity a l ->
-                                                        B.AMQ_available_capacity (AMQ_state_map a) l.
+                                                    B.AMQ_valid (AMQ_state_map a).
+    Axiom AMQ_map_capacityE: forall (a: A.AMQState p) l, A.AMQ_available_capacity h a l ->
+                                                         B.AMQ_available_capacity h (AMQ_state_map a) l.
 
-    Axiom AMQ_map_add_internalE: forall (a: A.AMQState p) val, A.AMQ_valid a -> A.AMQ_available_capacity a 1 ->
-      B.AMQ_add_internal (AMQ_state_map a) val = AMQ_state_map (@A.AMQ_add_internal _ h   a val).
+    Axiom AMQ_map_add_internalE: forall (a: A.AMQState p) val, A.AMQ_valid a -> A.AMQ_available_capacity h a 1 ->
+                                                               B.AMQ_add_internal (AMQ_state_map a) val = AMQ_state_map (@A.AMQ_add_internal _ h   a val).
 
-    Axiom AMQ_map_query_internalE: forall (a: A.AMQState p) val, A.AMQ_valid a -> A.AMQ_available_capacity a 1 ->
-      B.AMQ_query_internal (AMQ_state_map a) val = @A.AMQ_query_internal _ h a val.
+    Axiom AMQ_map_query_internalE: forall (a: A.AMQState p) val, A.AMQ_valid a -> A.AMQ_available_capacity h a 1 ->
+                                                                 B.AMQ_query_internal (AMQ_state_map a) val = @A.AMQ_query_internal _ h a val.
 
     Axiom AMQ_map_newE: forall (a: A.AMQState p), 
-      B.AMQ_new (AMQ_param_map p)  = AMQ_state_map (A.AMQ_new p).
+        B.AMQ_new (AMQ_param_map p)  = AMQ_state_map (A.AMQ_new p).
 
-   End Map.
+  End Map.
 End AMQMAP.
 
 Module AMQPropertyMap (AmqHash: AMQHASH) (A: AMQ AmqHash) (B: AMQ AmqHash) (Map: AMQMAP AmqHash A B) (Properties: AMQProperties AmqHash B) <:  AMQProperties AmqHash A.
@@ -622,7 +631,7 @@ Module AMQPropertyMap (AmqHash: AMQHASH) (A: AMQ AmqHash) (B: AMQ AmqHash) (Map:
       Properties.AMQ_false_positive_probability h (Map.AMQ_param_map s) n.
 
     Lemma AMQ_map_add_multipleE cbf hashes values f
-          (Hvalid: A.AMQ_valid cbf) (Hcap: A.AMQ_available_capacity cbf (length values)) :
+          (Hvalid: A.AMQ_valid cbf) (Hcap: A.AMQ_available_capacity h cbf (length values)) :
       \sum_(hshs in [finType of AmqHash.AMQHash h]) \sum_(cbf' in [finType of A.AMQState s])
        ((d[ AmqOperations.AMQ_add_multiple hashes cbf values]) (hshs,cbf') *R*
         (f hshs (Map.AMQ_state_map cbf'))) =
@@ -644,7 +653,7 @@ Module AMQPropertyMap (AmqHash: AMQHASH) (A: AMQ AmqHash) (B: AMQ AmqHash) (Map:
           rewrite -mulRA; apply f_equal.
           rewrite [_ *R* f _ _ ]mulRC; apply f_equal.
           apply f_equal => //=.
-          by rewrite -eqE eq_sym.
+            by rewrite -eqE eq_sym.
         }
       - {
           apply Logic.eq_sym => //=.
@@ -656,36 +665,36 @@ Module AMQPropertyMap (AmqHash: AMQHASH) (A: AMQ AmqHash) (B: AMQ AmqHash) (Map:
 
             under (@eq_bigr _ _ _ [finType of B.AMQState (Map.AMQ_param_map s)]) =>  bf' _. {
               suff <-:
-                 \sum_(i in [finType of AmqHash.AMQHash h])
-                 \sum_(i0 in [finType of _] | Map.AMQ_state_map i0 == bf')
-                 (FDistBind.d (d[ AmqHash.AMQHash_hash i val])
-                              (fun b : AmqHash.AMQHash h * AmqHash.AMQHashValue h =>
-                                 d[ let (new_hashes, hash_vec) := b in
-                                    ret (new_hashes, B.AMQ_add_internal bf' hash_vec)]) 
-                              (hshs', bf) *R*
-                  P[ AmqOperations.AMQ_add_multiple hashes cbf values === (i, i0)]) =
-            \sum_(i in AmqHash.AMQHash h)
-                 (P[ Properties.AmqOperations.AMQ_add_multiple hashes (Map.AMQ_state_map cbf) values === (i, bf')] *R*
-                  FDistBind.d (d[ AmqHash.AMQHash_hash i val])
-                              (fun b : AmqHash.AMQHash h * AmqHash.AMQHashValue h =>
-                                 d[ let (new_hashes, hash_vec) := b in
-                                    ret (new_hashes, B.AMQ_add_internal bf' hash_vec)])
-                              (hshs', bf)); first by over.
-              have Hcap': A.AMQ_available_capacity cbf (length values); first by eapply A.AMQ_available_capacityW with (n:= (length values).+1) => //=.
-            move: (@IHval Hcap'
-                        bf' (fun (i: [finType of AmqHash.AMQHash h]) (bf': [finType of B.AMQState (Map.AMQ_param_map s)]) =>
-                               FDistBind.d (d[ AmqHash.AMQHash_hash i val])
-                                           (fun b : AmqHash.AMQHash h * AmqHash.AMQHashValue h =>
-                                              d[ let (new_hashes, hash_vec) := b in
-                                                 ret (new_hashes, B.AMQ_add_internal bf' hash_vec)]) (hshs',bf) )) => //=.
-            move=>-> //=.
-            have ->: ((index_enum (AmqHash.AMQHash h))) = (index_enum [finType of AmqHash.AMQHash h]); last by apply f_equal => //=.
-              by rewrite index_enum_simpl.
+                   \sum_(i in [finType of AmqHash.AMQHash h])
+                   \sum_(i0 in [finType of _] | Map.AMQ_state_map i0 == bf')
+                   (FDistBind.d (d[ AmqHash.AMQHash_hash i val])
+                                (fun b : AmqHash.AMQHash h * AmqHash.AMQHashValue h =>
+                                   d[ let (new_hashes, hash_vec) := b in
+                                      ret (new_hashes, B.AMQ_add_internal bf' hash_vec)]) 
+                                (hshs', bf) *R*
+                    P[ AmqOperations.AMQ_add_multiple hashes cbf values === (i, i0)]) =
+              \sum_(i in AmqHash.AMQHash h)
+               (P[ Properties.AmqOperations.AMQ_add_multiple hashes (Map.AMQ_state_map cbf) values === (i, bf')] *R*
+                FDistBind.d (d[ AmqHash.AMQHash_hash i val])
+                            (fun b : AmqHash.AMQHash h * AmqHash.AMQHashValue h =>
+                               d[ let (new_hashes, hash_vec) := b in
+                                  ret (new_hashes, B.AMQ_add_internal bf' hash_vec)])
+                            (hshs', bf)); first by over.
+              have Hcap': A.AMQ_available_capacity h cbf (length values); first by eapply A.AMQ_available_capacityW with (n:= (length values).+1) => //=.
+              move: (@IHval Hcap'
+                            bf' (fun (i: [finType of AmqHash.AMQHash h]) (bf': [finType of B.AMQState (Map.AMQ_param_map s)]) =>
+                                   FDistBind.d (d[ AmqHash.AMQHash_hash i val])
+                                               (fun b : AmqHash.AMQHash h * AmqHash.AMQHashValue h =>
+                                                  d[ let (new_hashes, hash_vec) := b in
+                                                     ret (new_hashes, B.AMQ_add_internal bf' hash_vec)]) (hshs',bf) )) => //=.
+              move=>-> //=.
+              have ->: ((index_enum (AmqHash.AMQHash h))) = (index_enum [finType of AmqHash.AMQHash h]); last by apply f_equal => //=.
+                by rewrite index_enum_simpl.
 
             }
             under eq_bigr =>  bf' _. {
               rewrite exchange_big //=.
-              by over.
+                by over.
             }
               by over.
           } 
@@ -729,7 +738,7 @@ Module AMQPropertyMap (AmqHash: AMQHASH) (A: AMQ AmqHash) (B: AMQ AmqHash) (Map:
 
     Theorem AMQ_no_false_negatives (hashes: AmqHash.AMQHash h)  (amq: A.AMQState s) l x xs:
       uniq (x :: xs) -> length xs == l ->
-      A.AMQ_valid amq -> A.AMQ_available_capacity amq l.+1 ->
+      A.AMQ_valid amq -> A.AMQ_available_capacity h amq l.+1 ->
 
       AmqHash.AMQHash_hashstate_valid hashes ->
       AmqHash.AMQHash_hashstate_available_capacity hashes l.+1 ->
@@ -750,7 +759,7 @@ Module AMQPropertyMap (AmqHash: AMQHASH) (A: AMQ AmqHash) (B: AMQ AmqHash) (Map:
       length values == l ->
       AmqHash.AMQHash_hashstate_valid hashes ->
       AmqHash.AMQHash_hashstate_available_capacity hashes (l.+1) ->
-      A.AMQ_available_capacity (A.AMQ_new s) l.+1 ->
+      A.AMQ_available_capacity h (A.AMQ_new s) l.+1 ->
       all (AmqHash.AMQHash_hashstate_unseen hashes) (value::values) ->
       uniq (value::values) ->
         d[ 
@@ -790,7 +799,7 @@ Module AMQPropertyMap (AmqHash: AMQHASH) (A: AMQ AmqHash) (B: AMQ AmqHash) (Map:
       under eq_bigr => inds'' _. {
         under eq_bigr => ind' _; first under eq_bigr
         => hsh'' _; first under eq_rsum_ne0 => amq' Hamq.
-        have H1: B.AMQ_available_capacity (B.AMQ_new (Map.AMQ_param_map s)) (l + 1). {
+        have H1: B.AMQ_available_capacity h (B.AMQ_new (Map.AMQ_param_map s)) (l + 1). {
           rewrite Map.AMQ_map_newE //=.
             by apply Map.AMQ_map_capacityE; rewrite addn1.
             exact (A.AMQ_new s).
@@ -842,7 +851,7 @@ Module AMQPropertyMap (AmqHash: AMQHASH) (A: AMQ AmqHash) (B: AMQ AmqHash) (Map:
       under eq_bigr => inds'' _. {
         under eq_bigr => ind' _; first under eq_bigr
         => hsh'' _; first under eq_rsum_ne0 => amq' Hamq.
-        have H1: A.AMQ_available_capacity (A.AMQ_new s) (l + 1);first by rewrite addn1.
+        have H1: A.AMQ_available_capacity h (A.AMQ_new s) (l + 1);first by rewrite addn1.
         move: (@AmqOperations.AMQ_add_multiple_properties_preserve
                  h s (AmqHash.AMQHash_hashstate_put hashes value hshs')
                  (A.AMQ_new s) amq' values hsh'' l 1
@@ -888,14 +897,14 @@ Module AMQPropertyMap (AmqHash: AMQHASH) (A: AMQ AmqHash) (B: AMQ AmqHash) (Map:
         under eq_bigr do rewrite (@Map.AMQ_map_newE _ (A.AMQ_new s)) //=;
         apply Logic.eq_sym.
 
-      have H1: A.AMQ_available_capacity (A.AMQ_new s) (length values). {
+      have H1: A.AMQ_available_capacity h (A.AMQ_new s) (length values). {
         move/eqP:Hlen ->; apply   A.AMQ_available_capacityW with (n:=l.+1) => //=.
           by apply A.AMQ_new_validT.
       }
       under eq_bigr => hshs'' _. {
         under eq_rsum_ne0 => amq' Hamq.
 
-        have H1': A.AMQ_available_capacity (A.AMQ_new s) (l + 1). {
+        have H1': A.AMQ_available_capacity h (A.AMQ_new s) (l + 1). {
           by rewrite addn1.
         }
         move: (@AmqOperations.AMQ_add_multiple_properties_preserve
@@ -1130,15 +1139,15 @@ Module BasicHashVec  (Spec:HashSpec) <: AMQHASH.
   Definition AMQHashParams := (nat * nat)%type. (* first elem is n, second is l *)
 
   Definition AMQHashValue (pair: AMQHashParams) : finType :=
-    [finType of (snd pair).-tuple ('I_Spec.Hash_size.+1)].
+    [finType of (snd pair).+1.-tuple ('I_Spec.Hash_size.+1)].
 
   Definition AMQHash (pair: AMQHashParams) :=
-    [finType of (snd pair).-tuple (HashVec.Hash.HashState (fst pair))].
+    [finType of (snd pair).+1.-tuple (HashVec.Hash.HashState (fst pair))].
 
   Section AMQHash.
     Variable p: AMQHashParams. 
     Definition AMQHash_probability (pair: AMQHashParams) : Rdefinitions.R :=
-      ((Rdefinitions.Rinv (Spec.Hash_size.+1)%:R) ^R^ (snd pair)).
+      ((Rdefinitions.Rinv (Spec.Hash_size.+1)%:R) ^R^ (snd pair).+1).
 
     Section HashProbability.
       Variable h: AMQHashParams.
@@ -1146,9 +1155,9 @@ Module BasicHashVec  (Spec:HashSpec) <: AMQHASH.
       Lemma AMQHash_hash_prob_valid:
         \sum_(v in  AMQHashValue h) (AMQHash_probability h) = 1.
       Proof.
-        rewrite/AMQHashValue/AMQHash_probability //=; rewrite bigsum_card_constE.
+        rewrite/AMQHashValue/AMQHash_probability; rewrite bigsum_card_constE.
         rewrite card_tuple card_ord.
-        rewrite -natRexp //= -expRM mulRV //=; first by rewrite Rfunctions.pow1.
+        rewrite -natRexp -expRM mulRV //=; first by rewrite Rfunctions.pow1 mulR1.
         by rewrite RIneq.INR_IZR_INZ; apply/eqP => //=.
       Qed.
     End HashProbability.
@@ -1159,30 +1168,30 @@ Module BasicHashVec  (Spec:HashSpec) <: AMQHASH.
                (hashstate: AMQHash p) (key: AMQHashKey)
                (value: AMQHashValue p) : AMQHash p :=
       Tuple (@HashVec.hash_vec_insert_length
-         (fst p) (snd p) key hashstate value).
+         (fst p) (snd p).+1 key hashstate value).
 
 
     (* boolean properties of hash states*)
     Definition AMQHash_hashstate_available_capacity
                (hashstate:AMQHash p) (l:nat) :bool :=
-      (@HashVec.hashes_have_free_spaces (snd p) (fst p) hashstate l).
+      (@HashVec.hashes_have_free_spaces (snd p).+1 (fst p) hashstate l).
 
     Definition  AMQHash_hashstate_valid (hashstate: AMQHash p) : bool := true.
 
     Definition AMQHash_hashstate_contains
                (hashstate: AMQHash p) (key: AMQHashKey)
                (value: AMQHashValue p) : bool :=
-      (@HashVec.hash_vec_contains_value (fst p) (snd p) key hashstate value).
+      (@HashVec.hash_vec_contains_value (fst p) (snd p).+1 key hashstate value).
 
     Definition AMQHash_hashstate_unseen
       (hashstate: AMQHash p) (key:AMQHashKey) : bool :=
-      (@HashVec.hashes_value_unseen (snd p) (fst p) hashstate key).
+      (@HashVec.hashes_value_unseen (snd p).+1 (fst p) hashstate key).
 
     (* probabilistic hash operation*)
     Definition AMQHash_hash
                (hashstate: AMQHash p)
                (key: AMQHashKey) : Comp [finType of (AMQHash p * AMQHashValue p)] :=
-      (@HashVec.hash_vec_int (fst p) (snd p) key hashstate).
+      (@HashVec.hash_vec_int (fst p) (snd p).+1 key hashstate).
 
     (* properties of deterministic hash state operations *)
     Section DeterministicOperations.
@@ -1289,3 +1298,416 @@ Module BasicHashVec  (Spec:HashSpec) <: AMQHASH.
 
   End AMQHash.    
 End BasicHashVec.
+
+
+Module BloomFilterAMQ (Spec: HashSpec).
+  Module BasicHashVec := BasicHashVec Spec.
+  Module BloomFilterDefinitions :=  BloomFilterDefinitions Spec.
+
+  Export BasicHashVec.
+  Export BloomFilterDefinitions.
+
+  Module AMQ <: AMQ BasicHashVec.
+
+    Definition AMQStateParams := True.
+
+    Definition AMQState (val:AMQStateParams) : finType :=
+      [finType of BloomFilterDefinitions.BloomFilter ].
+
+    Section AMQ.
+      Variable p: AMQStateParams.
+      Variable h: BasicHashVec.AMQHashParams.
+
+      Definition AMQ_add_internal
+                 (amq: AMQState p)
+                 (inds: BasicHashVec.AMQHashValue h) : AMQState p :=
+        BloomFilterDefinitions.bloomfilter_add_internal
+          inds amq.
+
+      Definition AMQ_query_internal
+                 (amq: AMQState p) (inds: BasicHashVec.AMQHashValue h) : bool :=
+
+        BloomFilterDefinitions.bloomfilter_query_internal
+          inds amq.
+    Definition AMQ_available_capacity (_: BasicHashVec.AMQHashParams) (amq: AMQState p) (l:nat) : bool := true.
+    Definition AMQ_valid (amq: AMQState p) : bool := true.
+
+    Definition AMQ_new: AMQState p :=
+      BloomFilterDefinitions.bloomfilter_new.
+
+    
+    Lemma AMQ_new_nqueryE: forall vals, ~~ AMQ_query_internal  AMQ_new vals.
+    Proof.
+      move=> //= vals.
+      apply BloomFilterDefinitions.bloomfilter_new_empty.
+      by rewrite -length_sizeP size_tuple => //=.
+    Qed.
+    
+    Lemma AMQ_new_validT: AMQ_valid AMQ_new.
+    Proof.
+      by [].
+    Qed.
+    
+    Section DeterministicProperties.
+      Variable amq: AMQState p.
+
+      Lemma AMQ_available_capacityW: forall  n m,
+          AMQ_valid amq -> m <= n -> AMQ_available_capacity h amq n -> AMQ_available_capacity h amq m.
+      Proof.
+        by [].
+      Qed.
+      
+      Lemma AMQ_add_query_base: forall (amq: AMQState p) inds,
+        AMQ_valid amq -> AMQ_available_capacity h amq 1 ->
+        AMQ_query_internal (AMQ_add_internal amq inds) inds.
+      Proof.
+        move=> //= amq' inds _ _.
+        move: inds => [inds Hinds] //=.
+        rewrite/AMQ_query_internal/AMQ_add_internal//=; clear Hinds.
+        elim: inds  amq' => //= ind inds IHinds amq'.
+        apply/andP;split.
+        by apply bloomfilter_add_internal_preserve; apply tnth_set_nth_eq.
+        apply IHinds.
+      Qed.
+      
+    Lemma AMQ_add_valid_preserve: forall (amq: AMQState p) inds,
+        AMQ_valid amq -> AMQ_available_capacity h amq 1 ->
+        AMQ_valid (AMQ_add_internal amq inds).
+    Proof.
+      by [].
+    Qed.
+    
+    Lemma AMQ_add_query_preserve: forall (amq: AMQState p) inds inds',
+        AMQ_valid amq -> AMQ_available_capacity h amq 1 -> AMQ_query_internal amq inds ->
+        AMQ_query_internal (AMQ_add_internal amq inds') inds.
+    Proof.
+      move=> amq' inds inds' _ _.
+      move=>/allP Hquery; apply/allP => v Hv; move: (Hquery v Hv).
+      apply bloomfilter_add_internal_preserve.
+    Qed.
+    
+    Lemma AMQ_add_capacity_decr: forall (amq: AMQState p) inds l,
+        AMQ_valid amq -> AMQ_available_capacity h amq l.+1 ->
+        AMQ_available_capacity h (AMQ_add_internal amq inds) l.
+    Proof.
+      by [].
+    Qed.
+    
+    Lemma AMQ_query_valid_preserve: forall (amq: AMQState p) inds,
+        AMQ_valid amq -> AMQ_valid (AMQ_add_internal amq inds).
+    Proof.
+      by [].
+    Qed.
+    
+    Lemma AMQ_query_capacity_preserve: forall (amq: AMQState p) inds l,
+        AMQ_valid amq -> AMQ_available_capacity h amq l.+1 -> AMQ_available_capacity h (AMQ_add_internal amq inds) l.
+    Proof.
+      by [].
+    Qed.
+
+    End DeterministicProperties.
+  End AMQ.
+End AMQ.
+
+End BloomFilterAMQ.
+
+
+
+Module CountingBloomFilterAMQ (Spec: HashSpec).
+  Module BasicHashVec := BasicHashVec Spec.
+  Module CountingBloomFilterDefinitions :=  CountingBloomFilterDefinitions Spec.
+
+  Export BasicHashVec.
+  Export CountingBloomFilterDefinitions.
+
+  Module AMQ <: AMQ BasicHashVec.
+
+    Inductive AMQStateParamsInt :=
+      | mkStateParams (n:nat) of  n > 0.
+
+    Definition AMQStateParams := AMQStateParamsInt.
+
+    Definition AMQStateParamsToNat params :=
+      match params with
+      | mkStateParams n Hn => n
+      end.
+
+    Definition AMQState (n: AMQStateParams) : finType :=
+      [finType of CountingBloomFilterDefinitions.CountingBloomFilter (AMQStateParamsToNat n)].
+
+    Section AMQ.
+      Variable p: AMQStateParams.
+      Variable h: BasicHashVec.AMQHashParams.
+
+      Definition AMQ_add_internal
+                 (amq: AMQState p)
+                 (inds: BasicHashVec.AMQHashValue h) : AMQState p :=
+        CountingBloomFilterDefinitions.countingbloomfilter_add_internal
+          inds amq.
+
+      Definition AMQ_query_internal
+                 (amq: AMQState p) (inds: BasicHashVec.AMQHashValue h) : bool :=
+
+        CountingBloomFilterDefinitions.countingbloomfilter_query_internal
+          inds amq.
+
+
+
+      Definition AMQ_available_capacity (amq: AMQState p) (l:nat) : bool :=
+        CountingBloomFilterDefinitions.countingbloomfilter_free_capacity
+          amq (l * h.2.+1).
+
+
+
+    Definition AMQ_valid (amq: AMQState p) : bool := true.
+
+    Definition AMQ_new: AMQState p :=
+      CountingBloomFilterDefinitions.countingbloomfilter_new (AMQStateParamsToNat p).
+
+    
+    Lemma AMQ_new_nqueryE: forall vals, ~~ AMQ_query_internal  AMQ_new vals.
+    Proof.
+      move=> //= vals.
+      apply/allPn; exists (thead vals); first by apply mem_tnth.
+      rewrite/AMQ_new/countingbloomfilter_new.
+      move: (eq_ind_r _ _ _) => H1.
+      move: (@tnth_nseq_eq _ Hash_size.+1  (Ordinal (Hngt0 (AMQStateParamsToNat p))) (thead vals)).
+      rewrite/nseq_tuple.
+      move: (nseq_tupleP _ _) => H2.
+      rewrite (proof_irrelevance _ H1 H2); clear H1.
+      rewrite/countingbloomfilter_get_bit //= => -> //=.
+    Qed.
+    
+    Lemma AMQ_new_validT: AMQ_valid AMQ_new.
+    Proof.
+      by [].
+    Qed.
+    
+    Section DeterministicProperties.
+      Variable amq: AMQState p.
+
+      Lemma AMQ_available_capacityW: forall  n m,
+          AMQ_valid amq -> m <= n ->
+          AMQ_available_capacity amq n ->
+          AMQ_available_capacity amq m.
+      Proof.
+        move=> n m _ Hmn /allP Hcfb; apply/allP => v Hv.
+        move: (Hcfb v Hv).
+        move: Hmn; rewrite leq_eqVlt => /orP[/eqP -> | Hlmn] //=.
+        apply ltn_trans.
+        rewrite ltn_add2l ltn_mul2r //=.
+      Qed.
+      
+      Lemma AMQ_add_query_base: forall (amq: AMQState p) inds,
+        AMQ_valid amq -> AMQ_available_capacity amq 1 ->
+        AMQ_query_internal (AMQ_add_internal amq inds) inds.
+      Proof.
+        move=> //= amq' inds _ Hcap.
+        rewrite/  AMQ_query_internal/AMQ_add_internal.
+        apply countingbloomfilter_add_base.
+        move: inds => [inds Hinds] //=.
+        rewrite/AMQ_query_internal/AMQ_add_internal//=; clear Hinds.
+        by case: p => //=.
+      Qed.
+      
+      Lemma AMQ_add_valid_preserve: forall (amq: AMQState p) inds,
+        AMQ_valid amq -> AMQ_available_capacity amq 1 ->
+        AMQ_valid (AMQ_add_internal amq inds).
+      Proof.
+          by [].
+      Qed.
+    
+      Lemma AMQ_add_query_preserve: forall (amq: AMQState p) inds inds',
+        AMQ_valid amq -> AMQ_available_capacity amq 1 -> AMQ_query_internal amq inds ->
+        AMQ_query_internal (AMQ_add_internal amq inds') inds.
+    Proof.
+      move=> amq' inds inds' _ _.
+      apply countingbloomfilter_add_preserve.
+      by case p.
+    Qed.
+    
+    Lemma AMQ_add_capacity_decr: forall (amq: AMQState p) inds l,
+        AMQ_valid amq -> AMQ_available_capacity amq l.+1 ->
+        AMQ_available_capacity (AMQ_add_internal amq inds) l.
+    Proof.
+      rewrite/AMQ_available_capacity/AMQ_add_internal.
+      move=> amq' [inds Hinds] l _.
+      move:(@countingbloomfilter_add_capacity_change
+              0 _ h.2.+1 (l * h.2.+1) amq' inds Hinds
+           ).
+      by rewrite -mulSn => H /H //=.
+    Qed.
+    
+    Lemma AMQ_query_valid_preserve: forall (amq: AMQState p) inds,
+        AMQ_valid amq -> AMQ_valid (AMQ_add_internal amq inds).
+    Proof.
+      by [].
+    Qed.
+    
+    Lemma AMQ_query_capacity_preserve: forall (amq: AMQState p) inds l,
+        AMQ_valid amq -> AMQ_available_capacity amq l.+1 -> AMQ_available_capacity (AMQ_add_internal amq inds) l.
+    Proof.
+      apply AMQ_add_capacity_decr.
+    Qed.
+
+    End DeterministicProperties.
+    End AMQ.
+  End AMQ.
+  
+End  CountingBloomFilterAMQ.
+
+
+Module QuotientFilterAMQ (QSpec: QuotientFilterSpec).
+  Module QuotientFilterDefinitions := QuotientFilterDefinitions QSpec.
+
+  Module BasicHash := BasicHash  QuotientFilterDefinitions.QuotientHash.
+
+  Export BasicHash.
+  Export QuotientFilterDefinitions.
+
+  Module AMQ: AMQ BasicHash.
+
+
+  Definition AMQStateParams := True.
+  Definition AMQState (params: AMQStateParams) : finType :=
+    [finType of QuotientFilter].
+
+  Section AMQ.
+    Variable p: AMQStateParams.
+    Variable h: BasicHash.AMQHashParams.
+
+    Definition AMQ_add_internal
+      (amq: AMQState p) (value: BasicHash.AMQHashValue h):
+        AMQState p := quotientfilter_add_internal value amq.
+    
+    Definition AMQ_query_internal
+               (amq: AMQState p) (key: BasicHash.AMQHashValue h) : bool :=
+      quotientfilter_query_internal key amq.
+
+    Definition AMQ_available_capacity
+               (h: BasicHash.AMQHashParams) (amq: AMQState p) (l:nat): bool:=
+      quotientfilter_has_free_spaces (h.+1 * l) amq.
+
+    Definition AMQ_valid (amq:AMQState p) : bool :=
+      quotientfilter_valid amq.
+
+    Definition AMQ_new: AMQState p := quotientfilter_new.
+
+    Lemma AMQ_new_nqueryE: forall vals, ~~ AMQ_query_internal  AMQ_new vals.
+    Proof.
+      move=> vals; rewrite/AMQ_query_internal/quotientfilter_query_internal//=.
+      rewrite tnth_nseq_eq.
+      rewrite/fixlist_contains //=.
+      apply/hasPn => v.
+      move: (@fixlist_empty_is_empty [eqType of 'I_r.+1] n.+1).
+      rewrite/fixlist_is_empty =>/eqP -> //=.
+    Qed.
+    
+    Lemma AMQ_new_validT: AMQ_valid AMQ_new.
+    Proof.
+      by apply quotientfilter_new_valid.
+    Qed.
+    
+    Section DeterministicProperties.
+      Variable amq: AMQState p.
+
+      Lemma AMQ_available_capacityW: forall  n m,
+          AMQ_valid amq -> m <= n -> AMQ_available_capacity h amq n -> AMQ_available_capacity h amq m.
+      Proof.
+        move=> n m Hvalid Hnm /allP Hvv; apply/allP => v Hv; move:(Hvv v Hv) => //=.
+        apply leq_trans; rewrite leq_add2l //=.
+        by rewrite leq_mul2l Hnm; apply/orP; right.
+      Qed.
+      End DeterministicProperties.
+
+      Section DeterministicProperties.
+      Variable amq: AMQState p.
+
+      Lemma AMQ_add_query_base: forall (amq: AMQState p) inds,
+          AMQ_valid amq -> AMQ_available_capacity h amq 1 ->
+          AMQ_query_internal (AMQ_add_internal amq inds) inds.
+      Proof.
+        apply quotientfilter_add_query_base.
+      Qed.
+      
+      Lemma AMQ_add_valid_preserve: forall (amq: AMQState p) inds,
+          AMQ_valid amq -> AMQ_available_capacity h amq 1 ->
+          AMQ_valid (AMQ_add_internal amq inds).
+      Proof.
+        rewrite /AMQ_available_capacity muln1/AMQHashValue/AMQ_valid.
+        rewrite/quotientfilter_valid/quotientfilter_has_free_spaces.
+        move=> [amq'] ind /allP Hvv /allP Hspace; apply /allP => v.
+        rewrite/AMQ_add_internal/quotientfilter_add_internal.
+        case_eq (quotient_num ind) => quot rem Heq.
+
+        have H f:  quotientfilter_state {|  quotientfilter_state := f |} = f; first by [].
+        rewrite !H.
+        move=>/tnthP [ quot' ].
+        case Hquot: (quot' != quot).
+        - rewrite tnth_set_nth_neq; first move=>->; last by [].
+          apply Hvv.
+          by apply mem_tnth.
+        - move/Bool.negb_true_iff: Hquot; rewrite Bool.negb_involutive => /eqP ->.
+          rewrite tnth_set_nth_eq; first move=>->; last by [].
+          apply fixlist_insert_preserves_top_heavy.
+          apply Hvv.
+          by apply mem_tnth.
+      Qed.
+
+      Lemma AMQ_add_query_preserve: forall (amq: AMQState p) inds inds',
+          AMQ_valid amq -> AMQ_available_capacity h amq 1 -> AMQ_query_internal amq inds ->
+          AMQ_query_internal (AMQ_add_internal amq inds') inds.
+      Proof.
+        move=> amq' ind inds' Hvalid Hcap.
+        by apply quotientfilter_add_query_preserve.
+      Qed.
+      
+      Lemma AMQ_add_capacity_decr: forall (amq: AMQState p) inds l,
+          AMQ_valid amq -> AMQ_available_capacity h amq l.+1 ->
+          AMQ_available_capacity h (AMQ_add_internal amq inds) l.
+      Proof.
+        move=> amq' ind l Hvalid Hcap.
+        rewrite /AMQ_available_capacity in Hcap.
+        have Hobv: 0 < h.+1 * l.+1; first by rewrite muln_gt0; apply/andP;split => //=.
+        move: (@quotientfilter_add_preserve
+                 _ Hobv amq'
+                 (quotientfilter_add_internal ind amq')
+                 ind Hvalid Hcap
+                 (Logic.eq_refl
+                    (quotientfilter_add_internal ind amq'))
+              ) => /andP [_ ].
+
+        rewrite/AMQ_available_capacity.
+        rewrite mulnS addnC addnS -pred_Sn.
+        move=>/allP Hvv; apply/allP => v Hv; move: (Hvv v Hv).
+        by rewrite addnA =>/leq_addr_weaken.
+      Qed.
+      
+
+      Lemma AMQ_query_capacity_preserve: forall (amq: AMQState p) inds l,
+          AMQ_valid amq -> AMQ_available_capacity h amq l.+1 -> AMQ_available_capacity h (AMQ_add_internal amq inds) l.
+      Proof.
+        move=> amq' ind l Hvalid Hcap.
+        rewrite /AMQ_available_capacity in Hcap.
+        have Hobv: 0 < h.+1 * l.+1; first by rewrite muln_gt0; apply/andP;split => //=.
+        move: (@quotientfilter_add_preserve
+                 _ Hobv amq'
+                 (quotientfilter_add_internal ind amq')
+                 ind Hvalid Hcap
+                 (Logic.eq_refl
+                    (quotientfilter_add_internal ind amq'))
+              ) => /andP [_ ].
+
+        rewrite/AMQ_available_capacity.
+        rewrite mulnS addnC addnS -pred_Sn.
+        move=>/allP Hvv; apply/allP => v Hv; move: (Hvv v Hv).
+        by rewrite addnA =>/leq_addr_weaken.
+      Qed.
+      
+
+
+    End DeterministicProperties.
+  End AMQ.
+
+End AMQ.
+
